WPDS/WPDS_Code.thy
@@ -8,7 +8,7 @@ lemma accepts_step_distrib:
   shows "\<^bold>\<Sum>{d * (dioidLTS.accepts ts finals (q1,w))| q1 d. (p,([a],d),q1) \<in> wts_to_monoidLTS ts} = dioidLTS.accepts ts finals (p,a#w)"
 proof -
   have "finite (wts_to_monoidLTS ts)"
-    by (simp add: WPDS.finite_wts)
+    by (simp add: finite_wts)
   then have "finite {(p, ([a], d), q1) | d q1. (p, ([a], d), q1) \<in> wts_to_monoidLTS ts}"
     by (rule rev_finite_subset) auto
   then have "finite ((\<lambda>(p, (a, d), q1). (q1, d)) ` {(p, ([a], d), q1) |d q1. (p, ([a], d), q1) \<in> wts_to_monoidLTS ts})"
@@ -57,8 +57,6 @@ proof -
     by auto
 qed
 
-
-
 fun accepts_code :: "('state \<times> 'label \<times> 'state) \<Rightarrow>f 'weight::bounded_idempotent_semiring \<Rightarrow> 'state set \<Rightarrow> ('state \<times> 'label list) \<Rightarrow> 'weight"  where
     "accepts_code ts finals (p,[]) = (if p \<in> finals then 1 else 0)"
  |  "accepts_code ts finals (p,(y#w)) = (\<Sum>{(ts $ (p,y,q) * (accepts_code ts finals (q,w))) | q. ts $ (p,y,q) \<noteq> 0})"
@@ -66,7 +64,7 @@ fun accepts_code :: "('state \<times> 'label \<times> 'state) \<Rightarrow>f 'we
 lemma accepts_code_correct[code]:
   fixes ts :: "('state \<times> ('label::finite) \<times> ('state::enum)) \<Rightarrow>f 'weight::bounded_idempotent_semiring"
   fixes finals :: "'state set"
-  shows"dioidLTS.accepts ts finals (p,w) = accepts_code ts finals (p,w)"      
+  shows "dioidLTS.accepts ts finals (p,w) = accepts_code ts finals (p,w)"      
 proof (induction w arbitrary: p)
   case Nil
   then show ?case
@@ -103,12 +101,14 @@ locale WPDS_Code =
     and W :: "('ctr_loc, 'label) rule \<Rightarrow> 'weight::bounded_idempotent_semiring"
     and ts :: "(('ctr_loc, 'noninit::enum) state, 'label, 'weight::bounded_idempotent_semiring) w_transitions"
 begin
+
 definition "wrules = w_rules \<Delta> W"
 
-definition "checking rules A \<longleftrightarrow> (finite rules \<and> (\<forall>q. is_Init q \<longrightarrow> (\<forall>p \<gamma>. A $ (p, \<gamma>, q) = 0)))"
-lemma checking_implies: "checking \<Delta> ts \<Longrightarrow> WPDS_with_W_automata (w_rules \<Delta> W) ts"
+definition "checking \<longleftrightarrow> (finite \<Delta> \<and> (\<forall>q. is_Init q \<longrightarrow> (\<forall>p \<gamma>. ts $ (p, \<gamma>, q) = 0)))"
+
+lemma checking_implies: "checking \<Longrightarrow> WPDS_with_W_automata wrules ts"
   unfolding checking_def WPDS_with_W_automata_def finite_WPDS_def WPDS_with_W_automata_axioms_def 
-  using finite_w_rules by blast
+  using finite_w_rules unfolding wrules_def by blast
 
 
 definition "lbl = WPDS.lbl"
@@ -120,10 +120,11 @@ declare accept_pre_star_exec0'_def[code]
 
 thm WPDS_with_W_automata.pre_star_exec_correctness
 lemma pre_star_exec_correctness:
-  assumes "checking \<Delta> ts"
+  assumes "checking"
   shows "dioidLTS.accepts (WPDS_with_W_automata_no_assms.pre_star_exec' (w_rules \<Delta> W) ts) finals (Init p, w) =
-         dioidLTS.weight_pre_star (WPDS.transition_rel (w_rules \<Delta> W)) (\<lambda>(p, w). dioidLTS.accepts ts finals (Init p, w)) (p, w)"
-  using WPDS_with_W_automata.pre_star_exec_correctness[of "(w_rules \<Delta> W)" ts finals p w] checking_implies[OF assms] by blast
+         dioidLTS.weight_pre_star (WPDS.transition_rel wrules) (\<lambda>(p, w). dioidLTS.accepts ts finals (Init p, w)) (p, w)"
+  using WPDS_with_W_automata.pre_star_exec_correctness[of "wrules" ts finals p w] checking_implies[OF assms]
+  unfolding wrules_def by blast
 
 (*
 lemma augmented_WPDS_rules_code2[code]: "checking \<Delta> ts \<Longrightarrow> WPDS_with_W_automata_no_assms.augmented_WPDS_rules \<Delta> ts = (\<Union>((p, \<gamma>), d, (p', w)) \<in> \<Delta>. {((Init p, \<gamma>), d, (Init p', w))}) \<union> {((p,\<gamma>), d, (q, pop)) | p \<gamma> d q. ts $ (p,\<gamma>,q) = d}"
@@ -175,123 +176,10 @@ declare WPDS.lbl.simps[code]
 declare WPDS.accept_pre_star_exec0_def[code]
 declare Enum.enum_class.UNIV_enum[code]
 
-lemma update_wts_apply_is_1_if_member:
-  assumes "finite ts"
-  assumes "t' \<in> ts"
-  shows "update_wts (K$ 0) {(t, 1) |t. t \<in> ts} $ t' = (1 ::'weight::bounded_idempotent_semiring)"
-  using assms
-proof (induction rule: finite_induct)
-  case empty
-  then show ?case
-    by auto
-next
-  case (insert t'' F)
-  show ?case
-  proof (cases "t' = t''")
-    assume a: "t' = t''"
-    have "finfun_update_plus_pair (t'', 1) (update_wts (K$ 0) {(t, 1) |t. t \<in> F}) $ t' = (1 ::'weight::bounded_idempotent_semiring) + ((update_wts (K$ 0) {(t, 1) |t. t \<in> F}) $ t')"
-      by (simp add: a add.commute finfun_update_plus_pair_apply)
-    then have "finfun_update_plus_pair (t'', 1) (update_wts (K$ 0) {(t, 1) |t. t \<in> F}) $ t' = (1 ::'weight::bounded_idempotent_semiring)"
-      by (smt Collect_cong Groups.add_0 a empty_iff finfun_const_apply finite.emptyI fold_infinite insert.hyps(2) mem_Collect_eq prod.inject update_wts_def update_wts_empty update_wts_sum)
-    then have "update_wts (K$ 0) (insert (t'',1) {(t, 1) |t. t \<in> F}) $ t' = (1 ::'weight::bounded_idempotent_semiring)"
-      by (simp add: insert.hyps(1) update_wts_insert)
-    then show "update_wts (K$ 0) {(t, 1) |t. t \<in> insert t'' F} $ t' = (1 ::'weight::bounded_idempotent_semiring)"
-      by (smt (verit, del_insts) Collect_cong insert_Collect insert_iff)
-  next
-    assume a: "t' \<noteq> t''"
-    then have "t' \<in> F"
-      using insert by auto
-    then have "update_wts (K$ 0) {(t, 1) |t. t \<in> F} $ t' = (1 ::'weight::bounded_idempotent_semiring)"
-      using insert a by metis
-    then have "finfun_update_plus_pair (t'', 1) (update_wts (K$ 0) {(t, 1) |t. t \<in> F}) $ t' = (1 ::'weight::bounded_idempotent_semiring)"
-      by (simp add: a finfun_update_plus_pair_apply_other)
-    then have "update_wts (K$ 0) (insert (t'',1) {(t, 1) |t. t \<in> F}) $ t' = (1 ::'weight::bounded_idempotent_semiring)"
-      by (metis (no_types, lifting) insert(3) \<open>t' \<in> F\<close> finite_insert fold_infinite update_wts_def update_wts_insert)
-    then show "update_wts (K$ 0) {(t, 1) |t. t \<in> insert t'' F} $ t' = (1 ::'weight::bounded_idempotent_semiring)"
-      by (smt (verit, ccfv_SIG) Collect_cong insert_Collect insert_iff)
-  qed
-qed
-
-lemma update_wts_apply_is_0_if_not_member:
-  assumes "finite ts"
-  assumes "t' \<notin> ts"
-  shows "update_wts (K$ 0) {(t, 1) |t. t \<in> ts} $ t' = (0 ::'weight::bounded_idempotent_semiring)"
-  using assms
-proof (induction rule: finite_induct)
-  case empty
-  then show ?case
-    by (simp add: update_wts_empty)
-next
-  case (insert t'' F)
-  show ?case
-  proof (cases "t' = t''")
-    assume a: "t' = t''"
-    then show "update_wts (K$ 0) {(t, 1) |t. t \<in> insert t'' F} $ t' = (0 ::'weight::bounded_idempotent_semiring)"
-      using insert.prems by force
-  next
-    assume a: "t' \<noteq> t''"
-    then have "update_wts (K$ 0) {(t, 1) |t. t \<in> F} $ t' = (0 ::'weight::bounded_idempotent_semiring)"
-      using insert a by blast
-    then have "finfun_update_plus_pair (t'', 1) (update_wts (K$ 0) {(t, 1) |t. t \<in> F}) $ t' = (0 ::'weight::bounded_idempotent_semiring)"
-      by (simp add: a finfun_update_plus_pair_apply_other)
-    then have "update_wts (K$ 0) (insert (t'',1) {(t, 1) |t. t \<in> F}) $ t' = (0 ::'weight::bounded_idempotent_semiring)"
-      by (simp add: insert.hyps(1) update_wts_insert)
-    then show "update_wts (K$ 0) {(t, 1) |t. t \<in> insert t'' F} $ t' = (0 ::'weight::bounded_idempotent_semiring)"
-      by (smt (verit, ccfv_SIG) Collect_cong insert_Collect insert_iff)
-  qed
-qed
-
-lemma ts_to_wts_1_if_member:
-  assumes "finite ts"
-  assumes "(p', l, p'') \<in> ts"
-  shows "ts_to_wts ts $ (p', l, p'') = 1"
-  by (metis (mono_tags, lifting) assms ts_to_wts_def update_wts_apply_is_1_if_member)
-
-
-lemma ts_to_wts_1_or_0:
-  assumes "finite ts"
-  shows "ts_to_wts ts $ (p1, w, p2) = 1 \<or> ts_to_wts ts $ (p1, w, p2) = 0"
- using assms
-proof (induction rule: finite_induct)
-  case empty
-  then show ?case
-    by auto
-next
-  case (insert x F)
-  then show ?case
-  proof (cases "x =  (p1, w, p2)")
-    case True
-    then show ?thesis 
-      using insert
-      by (simp add: ts_to_wts_1_if_member)
-  next
-    case False
-    then show ?thesis 
-      using insert update_wts_apply_is_0_if_not_member update_wts_apply_is_1_if_member
-      by (metis (mono_tags) finite.insertI ts_to_wts_def)
-  qed    
-qed
-
-lemma ts_to_wts_bin:
-  assumes "finite ts"
-  shows "binary_aut (ts_to_wts ts)"
-  unfolding binary_aut_def using assms ts_to_wts_1_or_0 by metis
-
-lemma monoid_rtrancl_one_if_trans_star:
-  assumes "(p, v ::'label::finite list, q) \<in> LTS.trans_star ts"
-  assumes "finite ts"
-  shows "(p, (v, 1), q) \<in> monoid_rtrancl (wts_to_monoidLTS (ts_to_wts ts))"
-  apply (induction rule: LTS.trans_star.induct[OF assms(1)])
-  subgoal
-    apply (simp add: monoid_rtrancl_wts_to_monoidLTS_refl)
-    done
-  subgoal 
-    apply (metis ts_to_wts_1_if_member assms(2) monoid_rtrancl_intros_Cons mult.right_neutral wts_label_d wts_to_monoidLTS_exists)
-    done
-  done
 
 lemma accepts_1_if_monoid_rtrancl_1:
-  assumes "finite (ts :: ('s :: enum, 'd::finite) transition set)"
+  fixes ts :: "('s :: enum, 'l::finite) transition set"
+  assumes "finite ts"
   assumes "(p, (v, 1 :: 'weight), q) \<in> monoid_rtrancl (wts_to_monoidLTS (ts_to_wts ts))"
   assumes "q \<in> finals"
   shows "dioidLTS.accepts (ts_to_wts ts) finals (p, v) = (1::'weight::bounded_idempotent_semiring)"
@@ -321,19 +209,9 @@ proof -
     by (simp add: WPDS.accepts_def2)
 qed
 
-lemma ts_to_wts_not_member_is_0:
-  assumes "finite (ts :: (('ctr_loc::enum, 'noninit::enum) state, 'label::enum) transition set)"
-  assumes "(p, l, q) \<notin> ts"
-  shows "ts_to_wts ts $ (p, l, q) = 0"
-proof -
-  have f: "finite {(t, 1) |t. t \<in> ts}" using assms(1) by (fact finite_f_on_set)
-  show ?thesis
-    unfolding ts_to_wts_def update_wts_sum[OF f, of "K$ 0" "(p, l, q)"] using assms(2)
-    by simp
-qed
-
 lemma not_in_trans_star_implies_accepts_0:
-  assumes "finite (ts :: (('ctr_loc::enum, 'noninit::enum) state, 'label::enum) transition set)"
+  fixes ts :: "('s :: enum, 'label::enum) transition set"
+  assumes "finite ts"
   shows "\<forall>q\<in>finals. (p, w, q) \<notin> LTS.trans_star ts \<Longrightarrow> dioidLTS.accepts (ts_to_wts ts) finals (p, w) = (0::'weight::bounded_idempotent_semiring)"
 unfolding accepts_code_correct[of "ts_to_wts ts"]
 proof (induct w arbitrary: p)
@@ -361,7 +239,8 @@ next
 qed
 
 lemma lang_aut_is_accepts_full_new:
-  assumes "finite (ts :: (('ctr_loc::enum, 'noninit::enum) state, 'label::enum) transition set)"
+  fixes ts :: "(('ctr_loc::enum, 'noninit::enum) state, 'label::enum) transition set"
+  assumes "finite ts"
   shows "accepts_full (ts_to_wts ts) inits_set finals pv = (if pv \<in> P_Automaton.lang_aut ts Init finals then 1 else 0)"
   unfolding accepts_full_def P_Automaton.lang_aut_def P_Automaton.accepts_aut_def inits_set_def 
   apply simp
@@ -373,8 +252,10 @@ lemma lang_aut_is_accepts_full_new:
   using not_in_trans_star_implies_accepts_0[OF assms] by blast
 
 lemma weight_reach_set'_lang_aut_is_weight_reach'_accepts_full:
-  assumes "finite (ts :: (('ctr_loc::enum, 'noninit::enum) state, 'label::enum) transition set)"
-  assumes "finite (ts' :: (('ctr_loc::enum, 'noninit::enum) state, 'label::enum) transition set)"
+  fixes ts :: "(('ctr_loc::enum, 'noninit::enum) state, 'label::enum) transition set"
+  fixes ts' :: "(('ctr_loc, 'noninit) state, 'label) transition set"
+  assumes "finite ts"
+  assumes "finite ts'"
   shows "(WPDS.weight_reach_set' :: _ \<Rightarrow> _ \<Rightarrow> _ \<Rightarrow> 'weight::bounded_idempotent_semiring) (w_rules \<Delta> W) (P_Automaton.lang_aut ts Init finals) (P_Automaton.lang_aut ts' Init finals') =
          WPDS.weight_reach' (w_rules \<Delta> W) (accepts_full (ts_to_wts ts) inits_set finals) (accepts_full (ts_to_wts ts') inits_set finals')"
 proof -
@@ -392,6 +273,8 @@ proof -
 qed
 
 lemma WPDS_reach_exec_correct:
+  fixes ts :: "(('ctr_loc :: {card_UNIV,enum}, 'noninit::{card_UNIV,enum}) state, 'label::enum) transition set"
+  fixes ts' :: "(('ctr_loc, 'noninit) state, 'label) transition set"
   assumes "run_WPDS_reach \<Delta> W ts ts' finals finals' = Some (w :: 'weight::bounded_idempotent_semiring)"
   shows "w = (WPDS.weight_reach_set' (w_rules \<Delta> W) (P_Automaton.lang_aut ts Init finals) (P_Automaton.lang_aut ts' Init finals'))"
   using assms big_good_correctness_code[of "ts_to_wts ts" "w_rules \<Delta> W" "ts_to_wts ts'" inits_set finals finals', OF binary_aut_ts_to_wts[of ts]]
